src/goose_lang/trusted/github_com/mit_pdos/go_mvcc/trusted_proph.v
@@ -1,7 +1,10 @@
-From Perennial.goose_lang Require Import lang notation.
+From Goose.github_com.mit_pdos.go_mvcc Require Import wrbuf.
+From Perennial.goose_lang Require Import lang notation prelude.
 
 Section goose_lang.
-Context {ext:ffi_syntax}.
+Context `{ffi_sem: ffi_semantics}.
+Context {ext_ty:ext_types ext}.
+
 Local Coercion Var' (s:string) : expr := Var s.
 
 Definition ActReadId : Z := 0.
@@ -9,22 +12,33 @@ Definition ActAbortId : Z := 1.
 Definition ActCommitId : Z := 2.
 
 Definition NewProph : val :=
-  λ: <>, NewProph.
+  λ: <>, goose_lang.NewProph.
 
 Definition ResolveRead : val :=
-  λ: "p" "tid" "key", ResolveProph "p" (#ActReadId, ("tid", "key")).
+  λ: "p" "tid" "key", goose_lang.ResolveProph "p" (#ActReadId, ("tid", "key")).
 
 Definition ResolveAbort : val :=
-  λ: "p" "tid", ResolveProph "p" (#ActAbortId, "tid").
+  λ: "p" "tid", goose_lang.ResolveProph "p" (#ActAbortId, "tid").
 
-(* FIXME implement this *)
 Definition WrbufToVal : val :=
-  λ: "w", #().
+  λ: "wrbuf",
+    (* Goose alloc lemmas are very wonky, and directly allocating a #() does not work.
+       So we allocate a 0 and then store #() in it... *)
+    let: "res" := ref #0 in
+    "res" <- #();;
+    let: "slice" := (struct.loadF WrBuf "ents" "wrbuf") in
+    forSlice (structTy WrEnt) (λ: "idx" "val",
+      let: "key" := Fst "val" in
+      let: "str" := Fst (Snd "val") in
+      let: "present" := Fst (Snd (Snd "val")) in
+      "res" <- ("key", "present", "str", !"res")
+    ) "slice";;
+    !"res".
 
 Definition ResolveCommit : val :=
   λ: "p" "tid" "wrbuf",
   let: "wrbufval" := WrbufToVal "wrbuf" in
-  ResolveProph "p" (#ActCommitId, ("tid", "wrbufval")).
+  goose_lang.ResolveProph "p" (#ActCommitId, ("tid", "wrbufval")).
 
 End goose_lang.
 
